wip

src/ftype/minmaxsum_ftype.lean
@@ -1,114 +1,120 @@
+-- Experimental/broken - nothing relies on this. 
+
 import .basic .induction .single 
 ----------------------------------------------------------------
 open_locale classical 
 noncomputable theory 
 
-
 namespace ftype 
 -- The operations needed on the ftype A.
 section minmax
 
-variables {α : ftype}{β : Type}[nonempty α][linear_order β]
+variables {α : ftype}[nonempty α]{β : Type}[linear_order β]
 
+--instance i : has_coe_to_sort (set α) := 
+--{S := ftype, coe := λ X, { E := X, fin := by {letI := α.fin, apply_instance }}}
+
+
+instance duh {γ : ftype} : fintype γ := by {letI := γ.fin, apply_instance} 
+
+instance i {γ : Type}[fintype γ]: has_coe_to_sort γ := 
+{ S := ftype , coe := λ X, { E := X, fin := _ } }
 -- Proving this stuff probably needs fintype etc for ftype. 
 
 
 /-- finds the argmin of f over all sets X satisfying P -/
-lemma exists_arg_max_over_subtype (P : set U → Prop)(hP : set.nonempty P) (f : { X : set U // P X } → α): 
+lemma exists_arg_max_over_subtype (P : set α)[nonempty P](f : P → β): 
   ∃ X, ∀ Y, f Y ≤ f X := 
 begin
-  letI := fintype_of U,
-  haveI : nonempty { X : set U // P X } := ⟨classical.subtype_of_exists hP⟩, 
-  from fintype.exists_max f, 
+  letI := fintype_of α,
+  from fintype.exists_max f,
 end
 
 /-- finds the argmin of f over all sets X satisfying P -/
-lemma exists_arg_min_over_subtype (P : set U → Prop)(hP : set.nonempty P) (f : { X : set U // P X } → α): 
+lemma exists_arg_min_over_subtype (P : set α)[nonempty P] (f : P → β): 
   ∃ X, ∀ Y, f X ≤ f Y := 
-let f' : _ → (order_dual α) := f in exists_arg_max_over_subtype P hP f'
-
+let f' : _ → (order_dual β) := f in exists_arg_max_over_subtype P f'
 
 /-- maximum value of f over subsets of U satisfying P -/
-def arg_max_over (P : set U → Prop)(hP : set.nonempty P)(f : set U → α) : set U := 
-  (classical.some (exists_arg_max_over_subtype P hP (λ X, f X.val))).val 
+def arg_max_over (P : set α)[nonempty P](f : α → β) : α := 
+  (classical.some (exists_arg_max_over_subtype P (λ x, f x.val))).val 
 
 /-- subset of U attaining maximum value of f subject to satisfying P -/
-def max_val_over (P : set U → Prop)(hP : set.nonempty P)(f : set U → α) : α := 
-  f (arg_max_over P hP f)
+def max_val_over (P : set α)[nonempty P](f : α → β) : β := 
+  f (arg_max_over P f)
 
-lemma max_over_is_ub (P : set U → Prop)(hP : set.nonempty P)(f : set U → α):
-  ∀ X, P X → f X ≤ max_val_over P hP f :=
-λ X hX, classical.some_spec (exists_arg_max_over_subtype P hP (λ X, f X.val)) ⟨X, hX⟩
+lemma max_over_is_ub (P : set α)[nonempty P](f : α → β):
+  ∀ X, P X → f X ≤ max_val_over P f :=
+λ X hX, classical.some_spec (exists_arg_max_over_subtype P (λ X, f X.val)) ⟨X, hX⟩
   
-lemma arg_max_over_attains (P : set U → Prop)(hP : set.nonempty P)(f : set U → α):
-  P (arg_max_over P hP f) ∧ f (arg_max_over P hP f) = max_val_over P hP f := 
-let X' := (classical.some (exists_arg_max_over_subtype P hP (λ X, f X.val))) in 
+lemma arg_max_over_attains (P : set α)[nonempty P](f : α → β):
+  P (arg_max_over P f) ∧ f (arg_max_over P f) = max_val_over P f := 
+let X' := (classical.some (exists_arg_max_over_subtype P (λ X, f X.val))) in 
 ⟨X'.property, rfl⟩  
 
-lemma max_over_spec (P : set U → Prop)(hP : set.nonempty P)(f : set U → α):
-  ∃ X, P X ∧ (f X = max_val_over P hP f) ∧ (∀ Y, P Y → f Y ≤ f X)  := 
-let prev := arg_max_over_attains P hP f in 
-⟨arg_max_over P hP f,⟨prev.1,prev.2,max_over_is_ub P hP f⟩⟩  
+lemma max_over_spec (P : set α)[nonempty P](f : α → β):
+  ∃ X, P X ∧ (f X = max_val_over P f) ∧ (∀ Y, P Y → f Y ≤ f X)  := 
+let prev := arg_max_over_attains P f in 
+⟨arg_max_over P f,⟨prev.1,prev.2,max_over_is_ub P f⟩⟩  
 
 /-- minimum value of f over subsets of U satisfying P -/
-def arg_min_over (P : set U → Prop)(hP : set.nonempty P)(f : set U → α) : set U :=  
-  (classical.some (exists_arg_min_over_subtype P hP (λ X, f X.val))).val 
+def arg_min_over (P : set α)[nonempty P](f : α → β) : α :=  
+  (classical.some (exists_arg_min_over_subtype P (λ X, f X.val))).val 
 
 /-- subset of U attaining minimum value of f subject to satisfying P -/
-def min_val_over (P : set U → Prop)(hP : set.nonempty P)(f : set U → α) : α := 
-  f (arg_min_over P hP f)
+def min_val_over (P : set α)[nonempty P](f : α → β) : β := 
+  f (arg_min_over P f)
 
 
+lemma min_over_is_lb (P : set α)[nonempty P](f : α → β):
+  ∀ X, P X → min_val_over P f ≤ f X := 
+λ X hX, classical.some_spec (exists_arg_min_over_subtype P (λ X, f X.val)) ⟨X, hX⟩
 
-lemma min_over_is_lb (P : set U → Prop)(hP : set.nonempty P)(f : set U → α):
-  ∀ X, P X → min_val_over P hP f ≤ f X := 
-λ X hX, classical.some_spec (exists_arg_min_over_subtype P hP (λ X, f X.val)) ⟨X, hX⟩
 
-
-lemma arg_min_over_attains (P : set U → Prop)(hP : set.nonempty P)(f : set U → α):
-  P (arg_min_over P hP f) ∧ f (arg_min_over P hP f) = min_val_over P hP f := 
-let X' := (classical.some (exists_arg_min_over_subtype P hP (λ X, f X.val))) in 
+lemma arg_min_over_attains (P : set α)[nonempty P](f : α → β):
+  P (arg_min_over P f) ∧ f (arg_min_over P f) = min_val_over P f := 
+let X' := (classical.some (exists_arg_min_over_subtype P (λ X, f X.val))) in 
 ⟨X'.property, rfl⟩    
 
-lemma min_over_spec (P : set U → Prop)(hP : set.nonempty P)(f : set U → α):
-  ∃ X, P X ∧ (f X = min_val_over P hP f) ∧ (∀ Y, P Y → f X ≤ f Y)   := 
-let prev := arg_min_over_attains P hP f in 
-⟨arg_min_over P hP f,⟨prev.1,prev.2,min_over_is_lb P hP f⟩⟩ 
+lemma min_over_spec (P : set α)[nonempty P](f : α → β):
+  ∃ X, P X ∧ (f X = min_val_over P f) ∧ (∀ Y, P Y → f X ≤ f Y)   := 
+let prev := arg_min_over_attains P f in 
+⟨arg_min_over P f,⟨prev.1,prev.2,min_over_is_lb P f⟩⟩ 
 ---- 
 
 /-- maximum value of f over subsets of U -/
-def max_val (f : set U → α) : α := max_val_over (λ X, true) ⟨∅, trivial⟩ f
+def max_val (f : α → β) : β := max_val_over univ f
 
 /-- subset of U attaining maximum value of f -/
-def arg_max (f : set U → α) : set U := arg_max_over (λ X, true) ⟨∅, trivial⟩ f
+def arg_max (f : α → β) : α := arg_max_over univ f
 
 /-- minimum value of f over subsets of U -/
-def min_val (f : set U → α) : α := min_val_over (λ X, true) ⟨∅, trivial⟩ f
+def min_val (f : α → β) : β := min_val_over univ f
 
 /-- subset of U attaining minimum value of f-/
-def arg_min (f : set U → α) : set U := arg_min_over (λ X, true) ⟨∅, trivial⟩ f
+def arg_min (f : α → β) : α := arg_min_over univ f
 
-lemma max_is_ub (f : set U → α): 
+lemma max_is_ub (f : α → β): 
   ∀ X, f X ≤ max_val f :=
-λ X, by {apply max_over_is_ub, trivial} 
+λ X, by {apply max_over_is_ub, trivial}
 
-lemma arg_max_attains (f : set U → α): 
+lemma arg_max_attains (f : α → β): 
   f (arg_max f) = max_val f :=
-(arg_max_over_attains _ _ _).2
+(arg_max_over_attains _ _).2
 
-lemma min_is_lb (f : set U → α) :
+lemma min_is_lb (f : α → β) :
   ∀ X, min_val f ≤ f X := 
 λ X, by {apply min_over_is_lb, trivial} 
 
-lemma arg_min_attains (f : set U → α) : 
+lemma arg_min_attains (f : α → β) : 
   f (arg_min f) = min_val f := 
-(arg_min_over_attains _ _ _).2
+(arg_min_over_attains _ _).2
 
-lemma min_spec (f : set U → α):
+lemma min_spec (f : α → β):
   ∃ X, (∀ Y, f X ≤ f Y) ∧ (f X = min_val f) := 
 ⟨arg_min f, ⟨min_is_lb f, arg_min_attains f⟩ ⟩  
 
-lemma max_spec (f : set U → α):
+lemma max_spec (f : α → β):
   ∃ X, (∀ Y, f Y ≤ f X) ∧ (f X = max_val f) := 
 ⟨arg_max f, ⟨max_is_ub f, arg_max_attains f⟩ ⟩
 
@@ -116,80 +122,80 @@ lemma max_spec (f : set U → α):
 -- size 
 
 /-- largest set satisfying P -/
-def arg_max_size_over (P : set U → Prop)(hP : set.nonempty P) : set U := 
-  arg_max_over P hP size  
+def arg_max_size_over (P : set (set α))[nonempty P] : set α := 
+  arg_max_over P size  
 
 /-- size of largest set satisfying P -/
-def max_size_over (P : set U → Prop)(hP : set.nonempty P): ℤ := 
-  size (arg_max_size_over P hP)
+def max_size_over (P : α → Prop)(hP : set.nonempty P): ℤ := 
+  size (arg_max_size_over P)
 
-lemma max_size_over_is_ub (P : set U → Prop)(hP : set.nonempty P):
-  ∀ X, P X → size X ≤ max_size_over P hP:=
-max_over_is_ub P hP size 
+lemma max_size_over_is_ub (P : α → Prop)(hP : set.nonempty P):
+  ∀ X, P X → size X ≤ max_size_over P:=
+max_over_is_ub P size 
   
-lemma arg_max_size_over_attains (P : set U → Prop)(hP : set.nonempty P):
-  P (arg_max_size_over P hP) ∧ size (arg_max_size_over P hP) = max_size_over P hP := 
-  arg_max_over_attains P hP size 
+lemma arg_max_size_over_attains (P : α → Prop)(hP : set.nonempty P):
+  P (arg_max_size_over P) ∧ size (arg_max_size_over P) = max_size_over P := 
+  arg_max_over_attains P size 
 
-lemma max_size_over_spec (P : set U → Prop)(hP : set.nonempty P):
-  ∃ X, P X ∧ (size X = max_size_over P hP) ∧ (∀ Y, P Y → size Y ≤ size X)  := 
-  max_over_spec P hP size 
+lemma max_size_over_spec (P : α → Prop)(hP : set.nonempty P):
+  ∃ X, P X ∧ (size X = max_size_over P) ∧ (∀ Y, P Y → size Y ≤ size X)  := 
+  max_over_spec P size 
 
 
 /-- smallest set satisfying P -/
-def arg_min_size_over (P : set U → Prop)(hP : set.nonempty P) : set U := 
-  arg_min_over P hP size  
+def arg_min_size_over (P : α → Prop)(hP : set.nonempty P) : α := 
+  arg_min_over P size  
 
 /-- size of smallest set satisfying P -/
-def min_size_over (P : set U → Prop)(hP : set.nonempty P): ℤ := 
-  size (arg_min_size_over P hP)
+def min_size_over (P : α → Prop)(hP : set.nonempty P): ℤ := 
+  size (arg_min_size_over P)
 
-lemma min_size_over_is_lb (P : set U → Prop)(hP : set.nonempty P):
-  ∀ X, P X → min_size_over P hP ≤ size X :=
-min_over_is_lb P hP size 
+lemma min_size_over_is_lb (P : α → Prop)(hP : set.nonempty P):
+  ∀ X, P X → min_size_over P ≤ size X :=
+min_over_is_lb P size 
   
-lemma arg_min_size_over_attains (P : set U → Prop)(hP : set.nonempty P):
-  P (arg_min_size_over P hP) ∧ size (arg_min_size_over P hP) = min_size_over P hP := 
-  arg_min_over_attains P hP size 
+lemma arg_min_size_over_attains (P : α → Prop)(hP : set.nonempty P):
+  P (arg_min_size_over P) ∧ size (arg_min_size_over P) = min_size_over P := 
+  arg_min_over_attains P size 
 
-lemma min_size_over_spec (P : set U → Prop)(hP : set.nonempty P):
-  ∃ X, P X ∧ (size X = min_size_over P hP) ∧ (∀ Y, P Y → size X ≤ size Y)  := 
-  min_over_spec P hP size 
+lemma min_size_over_spec (P : α → Prop)(hP : set.nonempty P):
+  ∃ X, P X ∧ (size X = min_size_over P) ∧ (∀ Y, P Y → size X ≤ size Y)  := 
+  min_over_spec P size 
 
 --- Monotonicity 
 
-lemma max_over_subset_le_max (P Q : set U → Prop)(hP : set.nonempty P)(f : set U → α)(hPQ : set.subset P Q): 
-   max_val_over P hP f ≤ max_val_over Q (set.nonempty.mono hPQ hP) f := 
+lemma max_over_subset_le_max (P Q : α → Prop)(hP : set.nonempty P)(f : α → β)(hPQ : set.subset P Q): 
+   max_val_over P f ≤ max_val_over Q (set.nonempty.mono hPQ hP) f := 
 begin
-  rcases max_over_spec P hP f with ⟨XP, hXP⟩, 
+  rcases max_over_spec P f with ⟨XP, hXP⟩, 
   rcases max_over_spec Q (set.nonempty.mono hPQ hP) f with ⟨XQ, hXQ⟩,
   rw [←hXP.2.1, ←hXQ.2.1], 
   from hXQ.2.2  _ (hPQ hXP.1),
 end
 
-lemma min_le_min_over_subset (P Q : set U → Prop)(hP : set.nonempty P)(f : set U → α)(hPQ : set.subset P Q):
-  min_val_over Q (set.nonempty.mono hPQ hP) f ≤ min_val_over P hP f := 
+lemma min_le_min_over_subset (P Q : α → Prop)(hP : set.nonempty P)(f : α → β)(hPQ : set.subset P Q):
+  min_val_over Q (set.nonempty.mono hPQ hP) f ≤ min_val_over P f := 
 begin
-  rcases min_over_spec P hP f with ⟨XP, hXP⟩, 
+  rcases min_over_spec P f with ⟨XP, hXP⟩, 
   rcases min_over_spec Q (set.nonempty.mono hPQ hP) f with ⟨XQ, hXQ⟩,
   rw [←hXP.2.1, ←hXQ.2.1], 
   from hXQ.2.2  _ (hPQ hXP.1),
 end
 
-lemma max_over_le_max_over_of_mono (P : set U → Prop)(hP : set.nonempty P)(f f' : set U → α)(hff' : ∀ X, f X ≤ f' X):
-  max_val_over P hP f ≤ max_val_over P hP f' := 
+lemma max_over_le_max_over_of_mono (P : α → Prop)(hP : set.nonempty P)(f f' : α → α)(hff' : ∀ X, f X ≤ f' X):
+  max_val_over P f ≤ max_val_over P f' := 
 begin
-  rcases max_over_spec P hP f with ⟨X,hX⟩, 
-  rcases max_over_spec P hP f' with ⟨X', hX'⟩, 
+  rcases max_over_spec P f with ⟨X,hX⟩, 
+  rcases max_over_spec P f' with ⟨X', hX'⟩, 
   rw [←hX.2.1, ←hX'.2.1], 
   from le_trans (hff' X) (hX'.2.2 _ hX.1), 
 end
 
-lemma min_over_le_min_over_of_mono (P : set U → Prop)(hP : set.nonempty P)(f f' : set U → α)(hff' : ∀ X, f X ≤ f' X):
-  min_val_over P hP f ≤ min_val_over P hP f' := 
+lemma min_over_le_min_over_of_mono (P : α → Prop)(hP : set.nonempty P)(f f' : α → α)(hff' : ∀ X, f X ≤ f' X):
+  min_val_over P f ≤ min_val_over P f' := 
 begin
-  rcases min_over_spec P hP f with ⟨X,hX⟩, 
-  rcases min_over_spec P hP f' with ⟨X', hX'⟩, 
+  rcases min_over_spec P f with ⟨X,hX⟩, 
+  rcases min_over_spec P f' with ⟨X', hX'⟩, 
   rw [←hX.2.1, ←hX'.2.1], 
   from le_trans (hX.2.2 X' hX'.1) (hff' _),
 end
